lean/Spacewave.lean
@@ -5,5 +5,6 @@ import Spacewave.SObject.ResolvedOps
 import Spacewave.SObject.State
 import Spacewave.SObject.Host
 import Spacewave.SObject.KeyRotation
+import Spacewave.SObject.Invite
 
 #assert_standard_axioms
